Tweaking monad laws based on Properness.

theories/Structures/MonadLaws.v
@@ -1,4 +1,5 @@
 Require Import ExtLib.Structures.Monads.
+Require Import ExtLib.Structures.Proper.
 Require Import Equivalence.
 
 Set Implicit Arguments.
@@ -7,6 +8,11 @@ Set Strict Implicit.
 Section MonadLaws.
   Variable m : Type -> Type.
   Variable M : Monad m.
+
+  (** This states when an element is a proper element under an equivalence
+   ** relation.
+   **)
+  Variable Proper_m : forall T, Proper T -> Proper (m T).
 
   (** This <= relation is a computational <= relation based on the ideas
    ** of domain theory. It generalizes the usual equivalence relation by,
@@ -18,78 +24,102 @@ Section MonadLaws.
   Variable mleq : forall {T}, (T -> T -> Prop) -> m T -> m T -> Prop.
 
   Class MonadOrder : Type :=
-  { me_refl   : forall T (e : T -> T -> Prop),
-    Reflexive e -> Reflexive (mleq e)
-  ; me_trans  : forall T (e : T -> T -> Prop),
-    Transitive e -> Transitive (mleq e)
-  ; me_ret    : forall T (e : T -> T -> Prop) x y,
-    e x y -> mleq e (ret x) (ret y)
+  { me_refl   : forall T {P : Proper T} (e : T -> T -> Prop),
+    PReflexive e -> PReflexive (mleq e)
+  ; me_trans  : forall T {P : Proper T} (e : T -> T -> Prop),
+    PTransitive e -> PTransitive (mleq e)
   }.
 
-  Definition meq {T} (leq : T -> T -> Prop) (a b : m T) :  Prop :=
-    mleq leq a b /\ mleq leq b a.
+  Section meq.
+    Context {T : Type} (leq : T -> T -> Prop) (P : Proper T).
 
-  Global Instance Reflexive_meq {T} (leq : T -> T -> Prop) {_ : Reflexive leq}
-    (_ : MonadOrder) : Reflexive (meq leq).
-  Proof.
-    split; eapply me_refl; eauto.
-  Qed.
+    Definition meq (a b : m T) :  Prop :=
+      mleq leq a b /\ mleq leq b a.
 
-  Global Instance Symmetric_meq {T} (leq : T -> T -> Prop)
-    (_ : MonadOrder) : Symmetric (meq leq).
-  Proof.
-    unfold meq; split; intuition; intuition.
-  Qed.
+    Variable MO : MonadOrder.
 
-  Global Instance Transitive_meq {T} (leq : T -> T -> Prop) {_ : Transitive leq}
-    (_ : MonadOrder) : Transitive (meq leq).
-  Proof.
-    split; unfold meq in *; intuition; eapply me_trans; try eassumption.
-  Qed.
+    Global Instance PReflexive_meq {_ : PReflexive leq} : PReflexive meq.
+    Proof.
+      split; eapply me_refl; eauto.
+    Qed.
+
+    Global Instance PSymmetric_meq : PSymmetric meq.
+    Proof.
+      unfold meq; split; intuition; intuition.
+    Qed.
+
+    Global Instance PTransitive_meq {_ : PTransitive leq} : PTransitive meq.
+    Proof.
+      split; unfold meq in *; intuition.
+      { eapply me_trans; [ | | | | eassumption | eassumption ]; eauto. }
+      { eapply me_trans; [ | | | | eassumption | eassumption ]; eauto. }
+    Qed.
+  End meq.
+
+  Instance Proper_arrow {A B : Type} {Pa : Proper A} {Pb : Proper B} : Proper (A -> B) :=
+  { proper := fun f => forall x, proper x -> proper (f x) }.
 
   (** TODO: The real question is whether all of these [eX] relations
    ** need to be reflexive and transitive. They don't seem to need to be
    ** for option monad, but the proofs would be more automatable if they
    ** were b/c I'd be able to rewrite.
    **)
+  (** Should anything here mention meq? It seems like everything should be mleq **)
   Class MonadLaws : Type :=
   { morder :> MonadOrder
   ; bind_of_return : forall A B (a:A) (f:A -> m B) (eB : B -> B -> Prop),
     meq eB (bind (ret a) f) (f a)
-  ; return_of_bind : forall A (aM:m A) (f:A -> m A) (eA : A -> A -> Prop),
-    Reflexive eA ->
+  ; return_of_bind : forall A (PA : Proper A) (aM:m A) (f:A -> m A) (eA : A -> A -> Prop),
+    PReflexive eA -> proper aM -> proper f ->
     (forall x, meq eA (f x) (ret x)) -> meq eA (bind aM f) aM
   ; bind_associativity :
-    forall A B C (aM:m A) (f:A -> m B) (g:B -> m C) (eC : C -> C -> Prop),
-      Reflexive eC -> Transitive eC ->
+    forall A B C (PA : Proper A) (Pb : Proper B) (PC : Proper C) (aM:m A) (f:A -> m B) (g:B -> m C) (eC : C -> C -> Prop),
+      PReflexive eC -> PTransitive eC -> proper aM -> proper f -> proper g ->
       meq eC (bind (bind aM f) g) (bind aM (fun a => bind (f a) g))
 
-  ; bind_parametric_hd_leq : forall A B c c' (f : A -> m B) (eA : A -> A -> Prop) (eB : B -> B -> Prop),
+  ; ret_respectful : forall A (P : Proper A) (eA : A -> A -> Prop), 
+    forall x y, eA x y -> mleq eA (ret x) (ret y)
+    
+  ; bind_respectful_hd_leq : forall A B c c' (f : A -> m B) (eA : A -> A -> Prop) (eB : B -> B -> Prop),
     mleq eA c c' ->
     mleq eB (bind c f) (bind c' f)
-  ; bind_parametric_tl_leq : forall A B (f g : A -> m B) (eB : B -> B -> Prop),
-    Reflexive eB ->
+  ; bind_respectful_tl_leq : forall A B (PB : Proper B) (f g : A -> m B) (eB : B -> B -> Prop),
+    PReflexive eB ->
     (forall a, mleq eB (f a) (g a)) ->
     forall c, mleq eB (bind c f) (bind c g)
 
+  ; ret_proper : forall T (P : Proper T) (x : T), proper x -> proper (ret x) 
+  ; bind_proper : forall A B (Pa : Proper A) (Pb : Proper B) c (f : A -> m B),
+    proper c -> proper f -> proper (bind c f)
   }.
 
-  Theorem bind_parametric_hd (ml : MonadLaws) : forall A B c c' (f : A -> m B)
+(**
+  Section meq_respectful.
+    Variable ml : MonadLaws.
+
+    Theorem ret_respectful : forall A (P : Proper A) (eA : A -> A -> Prop), 
+      PReflexive 
+      forall x y, eA x y -> meq (mleq) eA (ret x) (ret y).
+
+
+  Theorem bind_respectful_hd : forall A B c c' (f : A -> m B)
     (eA : A -> A -> Prop) (eB : B -> B -> Prop),
     meq eA c c' ->
     meq eB (bind c f) (bind c' f).
   Proof.
-    intros; intuition. destruct H; split; eapply bind_parametric_hd_leq; eauto.
+    intros; intuition. destruct H; split; eapply bind_respectful_hd_leq; eauto.
   Qed.
 
-  Theorem bind_parametric_tl (ml : MonadLaws) : forall A B (f g : A -> m B) (eB : B -> B -> Prop),
+  Theorem bind_respectful_tl : forall A B (f g : A -> m B) (eB : B -> B -> Prop),
     Reflexive eB ->
     (forall a, meq eB (f a) (g a)) ->
     forall c, meq eB (bind c f) (bind c g).
   Proof.
-    intros; intuition. split; eapply bind_parametric_tl_leq; eauto; intros; edestruct H0; eauto.
+    intros; intuition. split; eapply bind_respectful_tl_leq; eauto; intros; edestruct H0; eauto.
   Qed.
+**)
 
+(*
   Class MonadTLaws (n : Type -> Type) (nM : Monad n) (MT : MonadT m n) : Type :=
   { lift_ret  : forall T (x : T) (eT : T -> T -> Prop),
     Reflexive eT -> Transitive eT ->
@@ -102,6 +132,9 @@ Section MonadLaws.
   Class MonadStateLaws s (MS : MonadState s m) : Type :=
   { get_put : forall eA,
     meq eA (bind get put) (ret tt)
+  ; put_get : forall A (eA : A -> A -> Prop),
+    forall x f, meq eA (bind (put x) (fun _ => bind get f))
+                       (bind (put x) (fun _ => f x))
   }.
 
   Class MonadReaderLaws S (MS : MonadReader S m) : Type :=
@@ -110,6 +143,7 @@ Section MonadLaws.
   ; local_local : forall T (s s' : S -> S) (c : m T) eA,
     meq eA (local s (local s' c)) (local (fun x => s' (s x)) c)
   }.
+*)
 
   Class MonadZeroLaws (MZ : MonadZero m) : Type :=
   { bind_zero :
@@ -117,26 +151,26 @@ Section MonadLaws.
   }.
 
   Class MonadFixLaws (MF : MonadFix m) : Type :=
-  { mfix_monotonic : forall T U (F : (T -> m U) -> T -> m U),
-    (** This is [Proper] with the right relations **)
-    (forall R R',
-      (forall x, mleq (@eq _) (R x) (R' x)) ->
-      forall x, mleq (@eq _) (F R x) (F R' x)) ->
+  { mfix_monotonic : forall T U (PT : Proper T) (PU : Proper U) 
+    (F : (T -> m U) -> T -> m U),
+    proper F ->
     forall x, mleq (@eq _) (mfix F x) (F (mfix F) x)
   }.
 
 End MonadLaws.
 
+(*
 Hint Rewrite bind_of_return bind_associativity using (eauto with typeclass_instances) : monad_rw.
 (* Hint Rewrite lift_ret lift_bind get_put ask_local local_local bind_zero : monad_rw. *)
 
 Ltac monad_norm :=
   let tc := solve [ eauto with typeclass_instances ] in
   let tac :=
-    repeat (eapply bind_parametric_hd; [ tc | tc | ]);
-    repeat (eapply bind_parametric_tl; [ tc | tc | intros ]);
+    repeat (eapply bind_respectful_hd; [ tc | tc | ]);
+    repeat (eapply bind_respectful_tl; [ tc | tc | intros ]);
     repeat (rewrite return_of_bind; [ tc | tc | intros ]);
     try (autorewrite with monad_rw; intros)
   in
   try ( unfold liftM, liftM2 in * ) ;
   repeat progress tac.
+*)
