theories/Structures/Proper.v
@@ -1,0 +1,20 @@
+Set Implicit Arguments.
+Set Strict Implicit.
+
+Class Proper (T : Type) : Type :=
+  proper : T -> Prop.
+
+Section relations.
+  Context {T : Type} {P : Proper T} (R : T -> T -> Prop).
+
+
+  Class PReflexive : Prop :=
+    preflexive : forall x : T, proper x -> R x x.
+  
+  Class PSymmetric : Prop :=
+    psymmetric : forall x y, proper x -> proper y -> R x y -> R y x.
+
+  Class PTransitive : Prop :=
+    ptransitive : forall x y z, proper x -> proper y -> proper z ->
+      R x y -> R y z -> R x z.
+End relations.
